OpenFlow/List_Group.thy
@@ -1,0 +1,35 @@
+theory List_Group
+imports Main
+begin
+
+section{*List Group*}
+
+function (sequential) list_group_eq :: "'a list \<Rightarrow> 'a list list" where
+  "list_group_eq [] = []" |
+  "list_group_eq (x#xs) = [x # takeWhile (op = x) xs] @ list_group_eq (dropWhile (op = x) xs)"
+by pat_completeness auto
+termination list_group_eq
+apply (relation "measure (\<lambda>N. length N )")
+apply(simp_all add: le_imp_less_Suc length_dropWhile_le)
+done
+
+value "list_group_eq [1::int,2,2,2,3,1,4,5,5,5]"
+
+
+function (sequential) list_group_eq_key :: "('a \<Rightarrow> 'b) \<Rightarrow> 'a list \<Rightarrow> 'a list list" where
+  "list_group_eq_key _ [] = []" |
+  "list_group_eq_key f (x#xs) = [x # takeWhile (\<lambda>y. f x = f y) xs] @ list_group_eq_key f (dropWhile (\<lambda>y. f x = f y) xs)"
+by pat_completeness auto
+termination list_group_eq_key
+apply (relation "measure (\<lambda>(f,N). length N )")
+apply(simp_all add: le_imp_less_Suc length_dropWhile_le)
+done
+
+value "list_group_eq_key fst [(1::int, ''''), (2,''a''), (2,''b''), (2, ''c''), (3, ''c''), (1,''''), (4,'''')]"
+
+lemma "list_group_eq_key id xs = list_group_eq xs"
+apply(induction xs)
+ apply(simp_all add: id_def)
+by (smt append.simps(1) append.simps(2) dropWhile.simps(1) dropWhile.simps(2) dropWhile_cong list.sel(3) list_group_eq.elims list_group_eq_key.elims takeWhile_cong)
+
+end
