OpenFlow/Sort_Descending.thy
@@ -1,0 +1,30 @@
+theory Sort_Descending
+imports Main
+begin
+
+section{* sorting descending *}
+  context linorder
+  begin
+  fun sorted_descending :: "'a list \<Rightarrow> bool" where
+    "sorted_descending [] \<longleftrightarrow> True" |
+    "sorted_descending (a#as) \<longleftrightarrow> (\<forall>x \<in> set as. a \<ge> x) \<and> sorted_descending as"
+  
+  definition sort_descending_key :: "('b \<Rightarrow> 'a) \<Rightarrow> 'b list \<Rightarrow> 'b list" where
+    "sort_descending_key f xs \<equiv> rev (sort_key f xs)"
+  end
+  lemma sorted_descending_Cons: "sorted_descending (x#xs) \<longleftrightarrow> sorted_descending xs \<and> (\<forall>y\<in>set xs. y \<le> x)"
+  by(induction xs) auto
+  
+  lemma sorted_descending_tail: "sorted_descending (xs@[x]) \<longleftrightarrow> sorted_descending xs \<and> (\<forall>y\<in>set xs. x \<le> y)"
+  by(induction xs) auto
+  
+  lemma sorted_descending: "sorted_descending (rev xs) \<longleftrightarrow> sorted xs"
+  apply(induction xs)
+   apply(simp)
+  apply(simp add: sorted_Cons sorted_descending_tail)
+  done
+  
+  lemma sort_descending: "sorted_descending (sort_descending_key (\<lambda>x. x) xs)"
+    by(simp add: sort_descending_key_def sorted_descending)
+
+end
